Update docs (#649)

demos/tutorial.v
@@ -22,6 +22,232 @@
 ========
 Tutorial
 ========
+
+Welcome! This is a quick primer for designing circuits with Cava. We'll walk
+through a few small examples end-to-end. This tutorial assumes some familiarity
+with Coq syntax. Use Ctrl+down and Ctrl+up to step through the Coq code along
+with the tutorial.
+
+.. coq:: none
 |*)
 
-Check nat.
+Require Import Cava.Cava.
+Require Import Cava.CavaProperties.
+Import Circuit.Notations.
+
+(*|
+Example 1 : Inverter
+====================
+
+To start, let's define a 1-bit inverter.
+|*)
+
+Definition inverter
+           {signal : SignalType -> Type}
+           {semantics : Cava signal}
+  : Circuit (signal Bit) (signal Bit) :=
+  Comb inv.
+
+(*|
+A few things to notice here:
+
+* ``SignalType`` is Cava's type system. The inverter is parameterized over
+  ``signal``, which converts ``SignalType``\ s to Coq types. ``Bit`` is one
+  example of a ``SignalType``; we'll see more examples later on.
+* ``Comb`` is short for "combinational"; our inverter has no loops, registers,
+  or timing requirements, so it is a purely combinational circuit.
+* The inverter is also paramterized over ``semantics``, an instance of the
+  typeclass ``Cava``. This instance provides implementations of circuit
+  primitives, such as 1-bit logic gates. One primitive gate is a 1-bit inverter
+  ``inv``, so our inverter is just a simple invocation of the primitive.
+
+Normally, we'd write circuit definitions a little more concisely by writing them
+inside a ``Section`` that contains ``signal`` and ``semantics`` as context
+variables, like this:
+|*)
+
+Section WithCava.
+  Context {signal} {semantics : Cava signal}.
+
+  Definition inverter_concise : Circuit (signal Bit) (signal Bit)
+    := Comb inv.
+
+(*|
+For the rest of the circuit definitions in this tutorial, you can assume that
+we're inside the section and that every definition is parameterized over the
+``signal`` and ``semantics`` context variables.
+
+Back to our inverter. Let's take a closer look at the ``inv`` primitive.
+|*)
+
+  About inv.
+
+(*|
+You can see in the type signature ``signal Bit -> cava (signal Bit)`` that
+``inv`` is defined as a pure Coq function in terms of a monad called
+``cava``. The ``cava`` monad, like ``inv``, is provided by ``semantics``. The
+monad is used to capture sharing; it's semantically different in Cava to write::
+
+  x <- inv zero ;;
+  y <- inv zero ;;
+  xor2 x y
+
+than it is to write::
+
+  x <- inv zero ;;
+  xor2 x x
+
+Both expressions have the same meaning, and if we were using Gallina ``let``
+binders there would be no difference. But the generated circuit can use two
+wires for the first definition, and fork the same wire in the second. As circuit
+diagrams, this is the difference between::
+
+         +-----+      +-----+
+  0 -----| inv |------|     |
+         +-----+      | xor |----- out
+         +-----+      |     |
+  0 -----| inv |------|     |
+         +-----+      +-----+
+
+and::
+
+                        +-----+
+                    +---|     |
+                    |   | xor |---- out
+         +-----+    |   |     |
+  0 -----| inv |----+---|     |
+         +-----+        +-----+
+
+This difference isn't significant in determining what the value of ``out`` will
+be, but it can be very useful when trying to exercise fine-grained control over
+circuit layout and area! At a first approximation, you can think of a monadic
+bind (``_ <- _ ;; ...``) as *naming a wire* in the circuit graph.
+
+We could have represented sharing by describing circuit graphs with a list of
+nodes and edges. However, this is essentially the "machine code" of structural
+hardware descriptions, and is far too tedious a representation for humans to
+work with. The monadic-function abstraction allows human engineers to think
+about the functional behavior and composition of circuits at a more intuitive
+level.
+
+Parameterizing over the ``cava`` monad and primitive implementations allows us
+to use different instances of ``Cava`` to interpret the same circuit definition
+in different ways. One ``Cava`` instance generates netlists by adding and
+connecting wires in the background using a state monad. For circuit simulations
+and proofs of functional correctness, on the other hand, we don't care about
+sharing at all; these use no-op identity monad that acts the same as a ``let``
+binder.
+
+Let's use our ``inverter`` definition to see these two interpretations in
+action.
+
+.. coq:: none
+|*)
+
+End WithCava. (* end the section so we can plug in signal and semantics *)
+
+(*|
+First, let's generate a netlist. We need to define an interface that describes the
+circuit's input and output ports and behavior relative to the (global) clock and
+reset signals. Then we can compute a netlist (type ``CavaState``), which
+describes the full layout of the circuit in a way that can be easily translated
+to SystemVerilog.
+|*)
+
+(* netlist-generating semantics *)
+Existing Instance CavaCombinationalNet.
+
+Definition inverter_interface
+  := sequentialInterface "inverter_interface"
+     "clk" PositiveEdge "rst" PositiveEdge
+     [mkPort "i" Bit]
+     [mkPort "o" Bit]
+     [].
+
+Compute (makeCircuitNetlist inverter_interface inverter).
+
+(* A closer look at the circuit body *)
+Compute (makeCircuitNetlist inverter_interface inverter).(module).
+
+(*|
+You may notice that we're using something called ``sequentialInterface`` here,
+and referring to clock and reset signals, even though our inverter is a purely
+combinational circuit. We introduce timing in the netlist interface here in
+order to drive the circuit with multiple inputs over time, and to plug it in as
+a subcomponent of circuits that are not combinational.
+
+Now, let's simulate the circuit, which can be useful for testing and proving
+functional correctness. Here, we use the identity-monad interpretation. The
+``signal`` for this ``Cava`` instance is ``combType``, which interprets a
+``Bit`` simply as a Coq ``bool``. If we provide the three inputs
+``[true; false; true]`` to the circuit simulation function ``multistep``, we'll
+get ``[false; true; false]``:
+|*)
+
+(* identity-monad semantics *)
+Existing Instance CombinationalSemantics.
+
+Compute (simulate inverter [true; false; true]).
+Compute (simulate inverter [true; false; true; true; true; false]).
+
+(*|
+We can use the simulation to write proofs about the circuit. For instance, we
+can prove that ``inverter`` obeys a natural Coq specification:
+|*)
+
+Lemma inverter_correct (input : list bool) :
+  simulate inverter input = map negb input.
+Proof.
+  (* inline the circuit definition *)
+  cbv [inverter].
+
+  (* simplify simulate to create an expression in terms of Coq lists *)
+  autorewrite with push_simulate.
+
+  (* assert that the two List.map functions are equivalent *)
+  apply map_ext. intros.
+
+  (* inline the inv primitive (fun x => ret (negb x)) *)
+  cbn [inv CombinationalSemantics].
+
+  (* simplify the identity monad expressions *)
+  simpl_ident.
+
+  reflexivity.
+Qed.
+
+(*|
+We can even prove that composing two inverters is the same as doing
+nothing. Here, ``>==>`` is circuit composition (a Kleisli arrow). The proof
+structure is pretty similar.
+|*)
+
+Lemma inverter_idempotent (input : list bool) :
+  simulate (inverter >==> inverter) input = input.
+Proof.
+  cbv [inverter].
+  autorewrite with push_simulate.
+  rewrite map_map.
+  apply List.map_id_ext. intros.
+  cbn [inv CombinationalSemantics].
+  simpl_ident.
+  apply Bool.negb_involutive.
+Qed.
+
+(*|
+To summarize, there are three things you can do with Cava circuits:
+
+1. Define them (parameterized over an abstract ``Cava`` instance)
+2. Generate netlists for them using the ``CavaCombinationalNet`` instance and
+   the ``makeCircuitNetlist`` function. These netlists can then be translated into
+   SystemVerilog.
+3. Simulate them using ``simulate``, and prove things about the simulations, by
+   plugging in the ``CombinationalSemantics`` instance.
+
+In the next example, we'll try a slightly more complex circuit.
+
+Example 2 : 8-Bit xor
+=====================
+
+To be continued!
+|*)
